% !TEX root = ../oddp.tex

\subsection{The bar resolution}\label{ss:milnor} Recall the that the Milgram construction applied to a group $G$, yields a contractible augmented simplicial set $\EG$ with a free $G$-action:
\begin{align*}
	(\EG)_k &= G^{k+1}\\
	\d_i(g_0\dots g_k) &= (g_0\dots\hat{g}_i\dots g_k) \\
	\s_i(g_0\dots g_k) &= (g_0\dots g_i,g_i\dots g_k)
\end{align*}
We can regard $\EC_r$ as the union $\bigcup_n \chains(\Cyc_r)^{\ot n}$ (this filters $\EC_r$ by degree). Then, the inclusion of $\Cyc_r$ as the vertices of $\asimplex^{r-1}$ induces a map $\chains(\EC_r) \to \bigcup_n\chains(\asimplex^{r-1})^{\ot n}$ that sends a tuple $(a_0,a_1,\dots,a_k)$ to the generator $[a_0]\ot \ldots \ot [a_k]$. The composition
\[
\chains(\EC_r) \lra \bigcup_n\chains(\asimplex^{r-1})^{\ot n} \lra \Waug{r}
\]
is an equivariant chain map. We can describe the dual of this map as follows: A generator $(-1)^{s}\cdot c\cdot (a_0,\ldots,a_{q-1})$ is \emph{admissible} if 
\begin{itemize}
	\item The generator $(-1)^{s'}\cdot (c\cdot \tilde{r}!) [a_0,\ldots,a_{q-r}]$ is admissible and $[a_{q-r},\ldots,a_{k-1}]$ does not contain repetitions and $(-1)^{s'+s}$ computes the parity of this permutation.
	\item $q<r$, then $s$ is the sign of the permutation that orders $[a_0,\ldots,a_{q-1}]$, $c$ equals $\frac{\varphi(q)}{\tilde{r}!}$, the number $r-1$ does not belong to the word, and the word obtained after ordering it starts with an even entry and alternates even and odd entries.
\end{itemize}

%
 %This composition has a description analogous to the one used to define $\Psiom$, using the following suspension map:
%\[
%S(a_0,\dots,a_k) = \begin{cases}
	%(-1)^{\sign{\perm}} (a_{0},\dots,a_{k-r+1}) & \text{ if $k \geq r-1$} \\
	%\emptyset & \text{if $k = r-2$ and $a_i\neq a_j$ for all $i,j$} \\
	%0 & \text{otherwise.}
%\end{cases}
%\]
%where $\pi$ is the permutation that orders $(a_{k-r+1},\dots,a_{k})$. The image of $e_{-q}^{\vee}$ is the sum of all words $A = (a_0,\dots,a_{q-1})\in \cochains[-q] \EC_r$ such that
%\begin{itemize}
%\item none of the subwords of the form $(a_{q-1-\ell(r-1)},a_{q-1-(\ell-1)(r-1))}$ of length $r$ contains repeated elements,
%\item the only subword of the form $(a_0,\dots,a_{q-1-\ell(r-1)})$ of length smaller than $r$ becomes, after having been ordered, an increasing sequence that alternates even and odd entries different from $r-1$, starting with an even entry.
%\end{itemize}
%each word has the sign needed to order each of the subwords mentioned above, and the coefficient $\frac{\varphi(m)!}{(\tilde{r}!)^j}$ where $m$ is the length of the last of the subwords mentioned, and $j$ is the total number of subwords and $\varphi(m) = \lfloor\frac{r-m-1}{2}\rfloor$.
\begin{example} If $r=3$,
\begin{align*}
	\Psi^\vee(e_{-1}^\vee) &= (0)
	\\
	\Psi^\vee(e_{-2}^{\vee}) &= (0,1)-(1,0)
	\\
	\Psi^\vee(e_{-3}^{\vee}) &= (0,1,2) - (0,2,1)
\\
	\Psi^\vee(e_{-4}^{\vee}) &= (0,1,2,0) - (0,1,0,2) + (1,0,2,1) - (1,0,1,2)
\end{align*}
if $r= 5$,
\begin{align*}
	\Psi^\vee(e^\vee_{-1}) &= \frac{1}{2}\left((0) + (2)\right)
	\\
	\Psi^\vee(e^\vee_{-2}) &= \frac{1}{2}\left((0,1) - (1,0) + (0,3) - (3,0) + (2,3) + (3,2)\right)
	\\
	\Psi^\vee(e^\vee_{-3}) &= \frac{1}{2}\left((0,1,2) -(0,2,1) + (1,2,0) - (1,0,2) + (2,0,1) - (2,1,0)\right)
\end{align*}
$\Psi^\vee(e^\vee_{-4})$ is the signed sum of all permutations of $(0,1,2,3)$, so it has $24$ summands, again with coefficient $\frac{1}{2}$.
\end{example}

This map is different from the one obtained in \cite[Prop.~6.16]{brumfiel2023explicit}, and in fact that map cannot be used to construct $\Psiom$ following the recipy of Definition \ref{def:psiom}.


\subsection{The even prime}\label{ss:even} If $r= 2$ and $R=\bF_2$, then $\bigcup_n \chains(\partial \asimplex^1)^{\ot n}$ is isomorphic to the unnormalized chain complex of $\EC_2$, while both $\Waug{r}$ and $\Per{r}$ are isomorphic to the normalized chain complex of $\EC_2$. The quotient map $\uchains(\EC_2) \to \chains(\EC_2)$ induces therefore a map
\[
\chains(\partial \asimplex^1)^{\ot (n+1)} \lra \Per{r} \overset{=}{\lra} \Waug{r}
\]
and it is easy to see that they intertwines $\theta_j$ and $\theta$, for $j=0,1$.
\begin{remark}
	The combinatorics in pages 13 and 14 of \cite{medina2021fast_sq} translate here to the fact that the map from the unnormalized chains to the normalized chains is well-defined, i.e., to the fact that the degenerate simplices generate a subcomplex of the unnormalized chain complex.
\end{remark}