Let $\cube{n}$ be the poset of subsets of $\{0,1,\ldots,n\}$, which we identify with the comma category $[n]\uparrow \asimplexinj$. Under this identification the empty subset becomes the identity arrow $[n]\to [n]$ and the whole $\{0,1,\ldots,n\}$ becomes the arrow $[n]\to [-1]$. Consider the following inclusions:
\begin{itemize}
    %\item The inclusion $g_i^{\top}\colon \cube{1}\to \cube{n}$ of the edge $\{0,\ldots,\hat{i},\ldots,n\}\overset{d_i}{\to} [n-1]$.
    %\item The inclusion $g_i^{\bot}\colon \cube{1}\to \cube{n}$ of the edge $[0]\overset{d_i}{\to} [-1]$.
    \item The inclusion $f_i^{\top}\colon \cube{n-1}\to \cube{n}$ that sends a vertex $(b_0,\ldots,b_k)$ to the vertex $b_0',\ldots,b_k'$, where $b_j' = b_j$ if $b_j<i$, $b_j' = i$ if $b_{j-1}<j\leq b_j$ and $b_j' = b_j+1$ if $b_j\geq i$.
    \item The inclusion $f_i^{\bot}\colon \cube{n-1}\to \cube{n}$ that sends a vertex $(b_0,\ldots,b_k)$ to the vertex $b_0',\ldots,b_k'$ where $b'_j = b_j$ if $b_j<i$ and $b_j' = b_j+1$ if $b_j\geq i$.
\end{itemize}
If $F\colon \asimplexinj^{\op}\to \cC$ is a (lax) functor, then define $F_n$ as the composition
    \[
    [n]\uparrow \asimplexinj\to \asimplexinj^{\op}\to \cC
    \]
Given a cube $F$ in $\cC$, define the following subcubes:
\begin{align*}
    %F_{i}^{|,\top} &= F\circ g_i^{\top} &
    %F_{i}^{|,\bot} &= F\circ g_i^{\bot} &
    F_{i}^{\diamond,\top} &= F\circ f_i^{\top} &
    F_{i}^{\diamond,\bot} &= F\circ f_i^{\bot}    
\end{align*}
and the following maps
\begin{align*}
    d_i^{\top}\colon F([n])\overset{d_i} F[n-1]
\end{align*}
\begin{definition}
    A \emph{resolution of the diagonal $\Delta$} assigns to each cube $F$ of dimension $n$ in the category $\cC$ a homomorphism $\Theta(F)\colon \abel(F(\{0,\ldots,n\}))\to \abel(F(\emptyset))^{\otimes r}$ such that
    \[
        \sum_i \Theta(F_i^{\bot})\circ \abel(d_i^{\top}) - \abel(d_i^{\bot})\circ\Theta(F_i^{\top}) = \begin{cases}
        N\Theta(F) & \text{ if $n$ is odd} \\
        T\Theta(F) & \text{ if $n$ is even},
        \end{cases}
    \]
    and if $F$ has dimension zero, then $\Theta(F) = \abel(\Delta)$.
\end{definition}
\begin{remark}
    Suppose that $F$ is a cube in $\cC$ with $F(\{0,1,\ldots,n\}) = Y'\amalg Y''$ and $F'$ is the cube that results from $F$ by redefining $F'(\{0,1,\ldots,n\}) = Y'$ and $F''$ is the cube that results from $F$ by redefining $F''(\{0,1,\ldots,n\}) = Y''$. If $\Theta$ has been defined on $F'$ and $F''$, then one can extend $\Theta$ to $F$ defining $\Theta(F) = \Theta(F')\amalg \Theta(F'')$.
\end{remark}
